theories/Group.v
@@ -1,0 +1,87 @@
+From Nominal Require Export Prelude.
+
+(** *Group operations *)
+Class Neutral A := neutral : A.
+Hint Mode Neutral ! : typeclass_instances.
+Notation ε := neutral.
+
+Class Operator A := op: A → A → A.
+Hint Mode Operator ! : typeclass_instances.
+(* Instance: Params (@op) 2 := {}. *)
+Infix "+" := op : nominal_scope.
+Notation "(+)" := op (only parsing) : nominal_scope.
+Notation "(+ x )" := (op x) (only parsing) : nominal_scope.
+Notation "( x +)" := (λ y, op y x) (only parsing) : nominal_scope.
+
+Class Inverse A := inv : A → A.
+Hint Mode Inverse ! : typeclass_instances.
+(* Instance: Params (@inv) 1 := {}. *)
+Notation "- x" := (inv x) : nominal_scope.
+Notation "(-)" := inv (only parsing) : nominal_scope.
+Notation "x - y" := (x + (-y))%nom (only parsing) : nominal_scope.
+
+Section Group.
+  Context A `{Equiv A, !Equivalence(≡@{A}), Neutral A, Operator A, Inverse A}.
+
+  Class Group: Prop := {
+    group_assoc : ∀ x y z, x + (y + z) ≡@{A} (x + y) + z;
+    group_left_id : ∀ x, ε + x ≡@{A} x;
+    group_right_id : ∀ x, x + ε ≡@{A} x;
+    group_left_inv : ∀ x, (-x) + x ≡@{A} ε;
+    group_right_inv : ∀ x, x - x ≡@{A} ε;
+
+    group_setoid :> Equivalence(≡@{A});
+    group_op_proper :> Proper ((≡@{A}) ==> (≡@{A}) ==> (≡@{A})) (+);
+    group_inv_proper :> Proper ((≡@{A}) ==> (≡@{A})) (-)
+  }.
+End Group.
+
+Arguments group_assoc {A AEq NA OA IA GA}: rename.
+Arguments group_left_id {A AEq NA OA IA GA}: rename.
+Arguments group_right_id {A AEq NA OA IA GA}: rename.
+Arguments group_left_inv {A AEq NA OA IA GA}: rename.
+Arguments group_right_inv {A AEq NA OA IA GA}: rename.
+Arguments group_op_proper {A AEq NA OA IA GA}: rename.
+Arguments group_inv_proper {A AEq NA OA IA GA}: rename.
+
+Section GroupProperties.
+  Context `{Group G}.
+
+  Corollary group_inv_involutive (x: G): x ≡ --x.
+  Proof with auto.
+    rewrite <-group_left_id at 1; rewrite <-group_left_inv, <-group_assoc, group_left_inv, group_right_id...
+  Qed.
+
+  Corollary inv_neutral: ε ≡@{G} -ε.
+  Proof with auto.
+    rewrite <-group_left_inv at 2; rewrite group_right_id, <-group_inv_involutive...
+  Qed.
+
+  (* Corollary group_inv_inj (x y: G): x ≡ y → (-x) ≡ (-y). *)
+  (* Proof. apply group_inv_proper. Qed. *)
+End GroupProperties.
+
+(** *Group action *)
+Class Action `(Group A) X := action: A → X → X.
+(* Instance: Params (@action) 2 := {}. *)
+Infix "∙" := action (at level 60, right associativity) : nominal_scope.
+Notation "(∙)" := action (only parsing) : nominal_scope.
+Notation "(∙ x )" := (action x) (only parsing) : nominal_scope.
+Notation "( x ∙)" := (λ y, action y x) (only parsing): nominal_scope.
+
+Section GroupAction.
+  Context A X `{Group A, Action A X, Equiv X, !Equivalence(≡@{X})}.
+
+  Class GroupAction: Prop := {
+    action_id : ∀ (x: X), ε ∙ x ≡@{X} x;
+    action_compat: ∀ (p q: A) (r: X), p ∙ (q ∙ r) ≡@{X} (q + p) ∙ r;
+
+    (* action_group :> Group A; *)
+    action_setoid :> Equivalence(≡@{X});
+    action_proper :> Proper ((≡@{A}) ==> (≡@{X}) ==> (≡@{X})) (∙)
+  }.
+End GroupAction.
+
+Arguments action_compat {A X AEq NA OA IA GA ActAX XEq GActAX}: rename.
+Arguments action_id {A X AEq NA OA IA GA ActAX XEq GActAX}: rename.
+Arguments action_proper {A X AEq NA OA IA GA ActAX XEq GActAX}: rename.
