theories/Perm.v
@@ -1,0 +1,87 @@
+From stdpp Require Import list.
+From Nominal Require Export Name Group.
+
+Notation perm := (list (name * name)).
+
+Definition swap '(a,b) : name -> name :=
+  λ c, if decide (a = c) then b else if decide (b = c) then a else c.
+
+Definition perm_action (p: perm): name -> name :=
+  λ a, foldr swap a p.
+
+(* Swap & perm properties *)
+Lemma swap_id (a x: name): swap (a,a) x = x.
+Proof. simpl; case_decide; congruence. Qed.
+
+Lemma swap_involutive a x: swap a (swap a x) = x.
+Proof. destruct a; simpl; repeat case_decide; congruence. Qed.
+
+Lemma perm_action_app p q x: perm_action (p ++ q) x = perm_action p (perm_action q x).
+Proof. unfold perm_action; rewrite foldr_app; auto. Qed.
+
+Lemma perm_action_left_rev p x: perm_action (reverse p) (perm_action p x) = x.
+Proof with auto.
+  induction p.
+  - simpl...
+  - assert (HH1: ∀ a, a :: p = [a] ++ p)...
+    rewrite HH1, reverse_app, reverse_singleton, <-perm_action_app, <-app_assoc, 3?perm_action_app;
+      simpl; rewrite swap_involutive...
+Qed.
+
+Lemma perm_action_right_rev p: forall x, perm_action p (perm_action (reverse p) x) = x.
+Proof with auto.
+  induction p; intros.
+  - simpl...
+  - assert (HH1: ∀ a, a :: p = [a] ++ p)...
+    rewrite HH1, reverse_app, reverse_singleton, <-perm_action_app, <-app_assoc, 3?perm_action_app,
+    IHp; simpl; apply swap_involutive.
+Qed.
+
+(** *Permutation group  *)
+Instance perm_neutral: Neutral perm := @nil (name * name).
+Instance perm_operator: Operator perm := @app (name * name).
+Instance perm_inverse: Inverse perm := @reverse (name * name).
+Instance perm_equiv: Equiv perm := λ p q: perm, ∀ a: name, perm_action p a = perm_action q a.
+Instance perm_equivalence: Equivalence (≡@{perm}).
+Proof. repeat split; repeat intro; [symmetry | etransitivity]; eauto. Qed.
+
+Instance perm_group: Group perm.
+Proof with auto.
+  split; unfold op, perm_operator, neutral, perm_neutral, inv, perm_inverse,
+         equiv, perm_equiv in *; repeat intro...
+  - rewrite app_assoc...
+  - rewrite app_nil_r...
+  - rewrite perm_action_app, perm_action_left_rev...
+  - rewrite perm_action_app, perm_action_right_rev...
+  - typeclasses eauto.
+  - rewrite 2?perm_action_app; do 2 match goal with H : context[_ = _] |- _ => rewrite H end...
+  - transitivity (perm_action (reverse y) (perm_action x (perm_action (reverse x) a)));
+      [rewrite H, perm_action_left_rev | rewrite perm_action_right_rev]...
+Qed.
+
+(** *Permtutation Types *)
+Class PermAction X := action_perm :> Action perm_group X.
+Class Perm X `{XA: PermAction X, Equiv X} : Prop :=
+  perm_type :> @GroupAction perm X _ _ _ _ perm_group (@action_perm X XA) _.
+
+(* Permutation types properties *)
+Section PermTypeProperties.
+  Context `{Perm X}.
+
+  Lemma perm_left_inv (x: X) p: (-p) ∙ p ∙ x ≡ x.
+  Proof. rewrite action_compat, group_right_inv, action_id; auto. Qed.
+
+  Lemma perm_rigth_inv (x: X) p: p ∙ (-p) ∙ x ≡ x.
+  Proof. rewrite action_compat, group_left_inv, action_id; auto. Qed.
+
+  Lemma perm_iff (x y: X) p: p ∙ x ≡ y <-> x ≡ (-p) ∙ y.
+  Proof.
+    split; intros A; [rewrite <-A, perm_left_inv | rewrite A, perm_rigth_inv]; auto.
+  Qed.
+
+  Lemma perm_inj (x y: X) p: p ∙ x ≡ p ∙ y <-> x ≡ y.
+  Proof.
+    split; intros A; [apply perm_iff in A; rewrite <-(perm_left_inv y p) | rewrite A]; auto.
+  Qed.
+
+End PermTypeProperties.
