theories/Prelude.v
@@ -1,0 +1,16 @@
+From stdpp Require Export prelude.
+
+Global Hint Mode Equiv ! : typeclass_instances.
+
+(* Class LeftInv {A} (R : relation A) (i: A) (f: A -> A -> A) (inv: A -> A): Prop := *)
+(*   left_inv x : R (f (inv x) x) i. *)
+(* Class RightInv {A} (R : relation A) (i: A) (f: A -> A -> A) (inv: A -> A): Prop := *)
+(*   right_inv x : R (f x (inv x)) i. *)
+
+(* Global Arguments left_inv {_ _} _ _ _ {_} _ : assert. *)
+(* Global Arguments right_inv {_ _} _ _ _ {_} _ : assert. *)
+
+Declare Scope nominal_scope.
+Delimit Scope nominal_scope with nom.
+Open Scope nominal_scope.
+
